pull updated `CompM_itrees`
from https://github.com/DeepSpec/InteractionTrees/blob/7bb773007ca7ea3164f00495505888e6bf36b549/theories/ITreeSpec/CompM_ITrees.v

coq/handwritten/CryptolToCoq/CompM_ITrees.v
@@ -2,9 +2,12 @@
  *** A version of the computation monad using the option-set monad
  ***)
 
-From Coq Require Export Morphisms Setoid.
+From Coq Require Export Morphisms Setoid Program.Equality.
 From ITree Require Export ITree ITreeFacts.
 From Paco Require Import paco.
+
+Infix ">>=" := ITree.bind (at level 58, left associativity).
+Notation "m1 >> m2" := (m1 >>= fun _ => m2) (at level 58, left associativity).
 
 Variant SpecEvent (E:Type -> Type) (A:Type) : Type :=
 | Spec_vis : E A -> SpecEvent E A
@@ -12,6 +15,22 @@ Variant SpecEvent (E:Type -> Type) (A:Type) : Type :=
 | Spec_exists : SpecEvent E A
 .
 
+Inductive SpecEvent' (E : Type -> Type) : Type -> Type :=
+  | Spec_vis' A : E A -> SpecEvent' E A
+  | Spec_forall' A : SpecEvent' E A
+  | Spec_exists' A : SpecEvent' E A
+  | Spec_assume A : itree (SpecEvent' E) A -> SpecEvent' E unit.
+
+(*
+Inductive satisfiesF' {E A} (satisfies : itree (SpecEvent' E) A -> itree E A -> Prop) 
+  : itree' (SpecEvent' E) A -> itree' E A -> Prop :=
+| Satisfies_Assume 
+    (hypothesis : itree (SpecEvent' E) A) 
+    (conclusion : unit -> itree (SpecEvent' E) A) (tree : itree E A) :
+    (satisfiesF' satisfies (observe hypothesis) (observe tree) -> 
+     satisfiesF' satisfies (observe (conclusion tt)) (observe tree) ) ->
+    satisfiesF' satisfies (VisF (Spec_assume E A hypothesis) conclusion) (observe tree).
+*)
 Arguments Spec_vis {E A}.
 Arguments Spec_forall {E A}.
 Arguments Spec_exists {E A}.
@@ -44,6 +63,8 @@ Inductive satisfiesF {E A} (satisfies : itree_spec E A -> itree E A -> Prop)
     (exists x:X, satisfies (spec x) tree) ->
     satisfiesF satisfies (VisF Spec_exists spec) (observe tree)
 .
+
+Hint Constructors satisfiesF.
 
 Instance Proper_satisfies_satisfiesF {E A} :
   Proper (pointwise_relation _ (pointwise_relation _ Basics.impl) ==>
@@ -295,11 +316,254 @@ Proof.
     apply IHe. assumption. }
 Qed.
 
+Ltac simpobs x := apply simpobs in x.
 
-Lemma satisfies_eutt_spec E A (P1 P2:itree_spec E A) tree :
+Ltac weaken_bis Hb := match type of Hb with ?x ≅ ?y => assert (x ≈ y); try (rewrite Hb; reflexivity) end.
+
+Lemma satisfies_eutt_spec_tau_vis_aux: forall (E : Type -> Type) (A u : Type) (e : SpecEvent E u)
+                                         (k1 k2 : u -> itree (SpecEvent E) A),
+    (forall v : u, paco2 (eqit_ eq true true id) bot2 (k1 v) (k2 v)) ->
+    forall (r : itree_spec E A -> itree E A -> Prop) (tree0 : itree E A),
+      (forall (P1 P2 : itree_spec E A) (tree : itree E A),
+          satisfies P1 tree -> P1 ≈ P2 -> r P2 tree) ->
+      satisfiesF (upaco2 satisfies_ bot2) (VisF e k1) (observe tree0) ->
+      satisfiesF (upaco2 satisfies_ r) (VisF e k2) (observe tree0).
+Proof.
+  intros E A u e k1 k2 REL r tree0 CIH H.
+  dependent induction H.
+  - rewrite <- x. constructor. eapply IHsatisfiesF; eauto.
+  - rewrite <- x. constructor. intros. right. 
+    pclearbot. eapply CIH; eauto. apply H.
+  - rewrite <- x. constructor. right. pclearbot; eapply CIH; eauto.
+    apply H.
+  - rewrite <- x. constructor. destruct H as [x' Hx' ]. pclearbot.
+    exists x'. right. eapply CIH; eauto.
+Qed.
+
+Lemma satisfiesF_TauL: forall (E : Type -> Type) (A : Type) (t1 : itree (SpecEvent E) A) 
+                         (tree0 : itree E A),
+    satisfiesF (upaco2 satisfies_ bot2) (TauF t1) (observe tree0) ->
+    satisfiesF (upaco2 satisfies_ bot2) (observe t1) (observe tree0).
+Proof.
+  intros E A t1 tree0 H.
+  dependent induction H; auto.
+  - pclearbot. rewrite <- x. constructor. punfold H.
+  - rewrite <- x. constructor. eapply IHsatisfiesF; eauto.
+Qed.
+
+(* Requires coinduction because the forall and exist states *)
+Lemma satisfies_TauR:
+  forall (E : Type -> Type) (A : Type) (P : itree_spec E A) (t : itree E A),
+    satisfies P (Tau t) ->
+    satisfies P t.
+Proof.
+  intros E A. pcofix CIH. intros P t HP.
+  pfold. red.
+  punfold HP. red in HP. dependent induction HP; pclearbot; auto.
+  - rewrite <- x. constructor. pstep_reverse. eapply paco2_mon; eauto.
+    intuition.
+  - rewrite <- x. constructor. eapply IHHP; eauto.
+  - pstep_reverse. clear IHHP. eapply paco2_mon with (r := bot2); intuition.
+  - rewrite <- x0. cbn in x. constructor. right.
+    eapply CIH; eauto. pfold. red. cbn. rewrite <- x. pstep_reverse.
+  - rewrite <- x0. constructor. destruct H as [x' Hx']. pclearbot.
+    exists x'. right. eapply CIH. pfold. red. rewrite <- x. pstep_reverse.
+Qed.
+
+(* infinte forall exist chains *)
+  
+
+Lemma satisfies_eutt_spec_l E A (P1 P2:itree_spec E A) tree :
   satisfies P1 tree -> eutt eq P1 P2 -> satisfies P2 tree.
 Proof.
-Admitted.
+  revert P1 P2 tree. pcofix CIH. intros P1 P2 tree HP HP12.
+  punfold HP. red in HP. pfold. red. punfold HP12. red in HP12.
+  dependent induction HP.
+  - rewrite <- x. rewrite <- x0 in HP12. dependent induction HP12; auto.
+    + rewrite <- x. constructor.
+    + rewrite <- x. constructor. eapply IHHP12; eauto.
+  - pclearbot.
+    remember (observe P2) as oP2. clear HeqoP2 P2.
+    assert ((exists P2', oP2 = TauF P2') \/ (forall P2', oP2 <> TauF P2') ).
+    { destruct oP2; eauto; right; repeat intro; discriminate. }
+    rewrite <- x. rewrite <- x0 in HP12. clear x0 x.
+    destruct H0 as [ [P2' HP2'] | HP2' ].
+    + subst. constructor. right. eapply CIH; eauto. 
+      rewrite <- tau_eutt. setoid_rewrite <- tau_eutt at 3.
+      pfold. auto.
+    + inversion HP12; try (exfalso; eapply HP2'; eauto; fail); subst.
+       clear HP12. punfold H. red in H. 
+       dependent induction REL; intros; subst; 
+       try (exfalso; eapply HP2'; eauto; fail).
+       * constructor. rewrite <- x in H.
+         clear CIH HP2' x. dependent induction H; try constructor.
+         ++ rewrite <- x. constructor.
+         ++ rewrite <- x. constructor. apply IHsatisfiesF; auto.
+       * rewrite <- x in H. constructor. pclearbot. 
+         eapply satisfies_eutt_spec_tau_vis_aux; eauto.
+       * eapply IHREL; auto. rewrite <- x in H.
+         eapply satisfiesF_TauL; eauto.
+  - eapply IHHP; eauto. rewrite <- x in HP12. 
+    assert (Tau spec ≈ P2); try (pfold; auto; fail).
+    rewrite tau_eutt in H. punfold H.
+  - rewrite <- x. constructor. eapply IHHP; eauto.
+  - rewrite <- x. rewrite <- x0 in HP12. dependent induction HP12.
+    + rewrite <- x. constructor. pclearbot. intros.  right. eapply CIH; eauto.
+      apply H.
+    + rewrite <- x. constructor. eapply IHHP12; eauto.
+  - rewrite <- x0 in HP12. dependent induction HP12.
+    + rewrite <- x. constructor. pclearbot. intros. right. eapply CIH; eauto.
+      pfold. red. rewrite <- x1.
+      specialize (H x2). punfold H.
+    + rewrite <- x. constructor. eapply IHHP12; eauto.
+  - rewrite <- x0 in HP12. rewrite <- x. clear x tree. dependent induction HP12.
+    + rewrite <- x. constructor. destruct H as [x' Hx']. pclearbot.
+      exists x'. right. eapply CIH; eauto.
+    + rewrite <- x. constructor. eapply IHHP12; eauto.
+Qed.
+
+Lemma satisfies_eutt_spec_r E A (P:itree_spec E A) (t1 t2 : itree E A) :
+  satisfies P t1 -> t1 ≈ t2 -> satisfies P t2.
+Proof.
+  revert P t1 t2. pcofix CIH. intros P t1 t2 HP Ht12.
+  pfold. red. punfold Ht12. red in Ht12. punfold HP. red in HP.
+  dependent induction Ht12.
+  - rewrite <- x. rewrite <- x0 in HP. clear x x0.
+    dependent induction HP; auto;
+    try (rewrite <- x; auto).
+    + rewrite <- x0. pclearbot. constructor.
+      intros. right. eapply CIH; try apply H. reflexivity.
+    + rewrite <- x0. constructor. destruct H as [x' Hx']. pclearbot.
+      exists x'. right. eapply CIH; eauto. reflexivity.
+      (* Tau Tau case *)
+  - pclearbot. remember (observe P) as oP. clear HeqoP P.
+    assert ( (exists P, oP = TauF P) \/ (forall P, oP <> TauF P) ).
+    { destruct oP; eauto; right; repeat intro; discriminate. }
+    destruct H as [ [P HoP] | HoP].
+    + subst. rewrite <- x. constructor. right. eapply CIH; eauto.
+      apply satisfies_TauR. pfold. red. apply satisfiesF_TauL. simpl.
+      rewrite x0. auto.
+    + rewrite <- x. rewrite <- x0 in HP.
+      inversion HP; try (exfalso; eapply HoP; eauto; fail).
+      * subst. clear HP. clear x x0. punfold REL. red in REL. constructor.
+        dependent induction H1; try (exfalso; eapply HoP; eauto; fail).
+        ++ rewrite <- x in REL. clear x. dependent induction REL;
+           try (rewrite <- x; auto).
+        ++ eapply IHsatisfiesF; auto. pstep_reverse. 
+           assert (m1 ≈ m2); try (pfold; auto; fail). simpobs x. rewrite x in H.
+           rewrite tau_eutt in H. auto.
+        ++ rewrite <- x in REL. clear x. dependent induction REL.
+           ** rewrite <- x; auto. constructor. right. 
+              pclearbot. eapply CIH; eauto. apply H.
+           ** rewrite <- x. constructor. eapply IHREL; eauto.
+        ++ pclearbot. constructor. right. eapply CIH; eauto. pfold. red.
+           rewrite <- x. pstep_reverse.
+        ++ constructor. destruct H as [x' Hx']. pclearbot. exists x'. right.
+           eapply CIH; eauto. simpobs x. rewrite <- itree_eta in x. rewrite <- x.
+           pfold. auto.
+      * constructor. constructor. right. pclearbot. eapply CIH; eauto.
+        apply satisfies_TauR. pfold. red. cbn. rewrite <- H. pstep_reverse.
+      * constructor. constructor. destruct H1 as [x' Hx' ]. pclearbot.
+        exists x'. right. eapply CIH; eauto. symmetry in H. simpobs H.
+        rewrite H. rewrite tau_eutt. auto.
+  - rewrite <- x. rewrite <- x0 in HP. clear x x0. dependent induction HP.
+    + rewrite <- x. constructor. eapply IHHP; eauto.
+    + rewrite <- x. constructor. intros. right. 
+      pclearbot. eapply CIH; eauto. apply H.
+    + rewrite <- x0. pclearbot. 
+      assert (VisF e k2 = observe (Vis e k2) ); auto. rewrite H0.
+      constructor. intros. right. eapply CIH; try apply H.
+      symmetry in x. simpobs x. rewrite x.
+      pfold. red. constructor. auto.
+    + rewrite <- x0. assert (VisF e k2 = observe (Vis e k2) ); auto.
+      rewrite H0. constructor. destruct H as [x' Hx']. pclearbot.
+      exists x'. right. eapply CIH; eauto. symmetry in x. simpobs x.
+      rewrite x. pfold. constructor. left. auto.
+  - eapply IHHt12; auto. rewrite <- x in HP. pstep_reverse.
+    apply satisfies_TauR. pfold. auto.
+  - rewrite <- x. constructor. 
+    eapply IHHt12; eauto.
+Qed. 
+
+Instance proper_eutt_satisfies E R : Proper (@eutt (SpecEvent E) R R eq ==> eutt eq ==> iff) satisfies.
+Proof.
+  intros P Q HPQ t1 t2 Ht12. split; intros.
+  - eapply satisfies_eutt_spec_r; eauto. eapply satisfies_eutt_spec_l; eauto.
+  - symmetry in HPQ. symmetry in Ht12. eapply satisfies_eutt_spec_r; eauto. eapply satisfies_eutt_spec_l; eauto.
+Qed.
+
+CoFixpoint top_spec {E: Type -> Type} {A : Type} : itree_spec E A := Vis Spec_forall (fun _ : unit => top_spec).
+
+Lemma top_spec_is_top : forall E R (t : itree E R), satisfies top_spec t.
+Proof.
+  intros E R. pcofix CIH. intros. pfold. red. cbn. constructor. intros. right. auto.
+Qed.
+
+Definition bottom_spec {E : Type -> Type} {A : Type} : itree_spec E A := Vis Spec_exists (fun v : void => match v with end).
+
+Lemma bottom_spec_is_bottom : forall E R (t : itree E R), ~ satisfies bottom_spec t.
+Proof.
+  intros E R t Hcontra. punfold Hcontra. red in Hcontra. cbn in *. dependent induction Hcontra; eauto.
+  destruct H as [ [] _ ].
+Qed.
+
+Definition and_spec {E : Type -> Type} {A : Type} (P Q : itree_spec E A) :=
+  Vis Spec_forall (fun b : bool => if b then P else Q).
+
+Definition or_spec {E : Type -> Type} {A : Type} (P Q : itree_spec E A) :=
+  Vis Spec_exists (fun b : bool => if b then P else Q).
+
+Lemma and_spec_is_and : forall E R (t : itree E R) (P Q : itree_spec E R),
+    satisfies (and_spec P Q) t <-> (satisfies P t /\ satisfies Q t).
+Proof.
+  split; [split | idtac]; intros.
+  - punfold H. red in H. pfold. red. cbn in H. dependent induction H.
+    + rewrite <- x. constructor. eauto.
+    + simpobs x. rewrite <- itree_eta in x. pclearbot. pstep_reverse.
+      specialize (H true). cbn in *. rewrite x. auto.
+  - punfold H. red in H. pfold. red. cbn in H. dependent induction H.
+    + rewrite <- x. constructor. eauto.
+    + simpobs x. rewrite <- itree_eta in x. pclearbot. pstep_reverse.
+      specialize (H false). cbn in *. rewrite x. auto.
+  - destruct H. pfold. red. cbn. constructor. intros; destruct x; left; auto.
+Qed.
+
+Lemma or_spec_is_or : forall E R (t : itree E R) (P Q : itree_spec E R),
+    satisfies (or_spec P Q) t <-> (satisfies P t \/ satisfies Q t).
+Proof.
+  split; intros; [idtac | destruct H] .
+  - punfold H. red in H. cbn in *. dependent induction H; [ simpobs x | idtac ].
+    + setoid_rewrite x. setoid_rewrite tau_eutt. eapply IHsatisfiesF; eauto.
+    + simpobs x. rewrite <- itree_eta in x. setoid_rewrite x.
+      destruct H as [ [ | ] H ]; pclearbot; eauto.
+  - pfold. red. cbn. constructor. exists true. auto.
+  - pfold. red. cbn. constructor. exists false. auto.
+Qed.
+
+Lemma or_spec_bind : forall E R S (P Q : itree_spec E R) (k : R -> itree_spec E S),
+    (or_spec P Q) >>= k ≈ or_spec (P >>= k) (Q >>= k).
+Proof.
+  intros. unfold or_spec. rewrite bind_vis. pfold. constructor.
+  intros; left.
+  enough ( (if v then P else Q) >>= k ≈ if v then P >>= k else Q >>= k ); auto.
+  destruct v; reflexivity.
+Qed.
+
+Lemma and_spec_bind : forall E R S (P Q : itree_spec E R) (k : R -> itree_spec E S),
+    (and_spec P Q) >>= k ≈ and_spec (P >>= k) (Q >>= k).
+Proof.
+  intros. unfold and_spec.
+  pfold. red. cbn. constructor.
+  intros; left.
+  enough ( (if v then P else Q) >>= k ≈ if v then P >>= k else Q >>= k ); auto.
+  destruct v; reflexivity.
+Qed.
+
+(*
+Definition imp_spec {E R} (P Q : itree_spec E R) := 
+  Vis Spec_forall (fun _ : satisfies P t => Q)
+*)
+
 (*
   revert P1 P2 tree; pcofix CIH; intros P1 P2 tree sats e12.
   destruct (eutt_split _ _ _ _ e12) as [ P1' e1 [ P2' e2 e12' ]].
@@ -447,16 +711,19 @@ pinversion sats. Focus 2.
 Qed.
 *)
 
-
+(*
 Instance Proper_eutt_satisfies E A : Proper (eutt eq ==> eutt eq ==> iff) (@satisfies E A).
 Proof.
 Admitted.
 
+(* in general I think lemmas like htese are false, like let r be strong bisimulation and consider examples *)
+(* cofix t1 := Vis e (fun _ => t1)  cofix t2 := Tau (Vis e (fun _ => t2) ) *)
+(* You can take a vis step, *)
 Instance Proper_eutt_satisfiesF E A r : Proper (eutt eq ==> eutt eq ==> iff)
                                                (paco2 (@satisfies_ E A) r).
 Proof.
-Admitted.
-
+Abort.
+*)
 (* The proposition that a is returned by an itree along some path *)
 Inductive is_itree_retval' {E A} : itree' E A -> A -> Prop :=
 | iirv_ret a : is_itree_retval' (RetF a) a
@@ -468,10 +735,6 @@ Inductive is_itree_retval' {E A} : itree' E A -> A -> Prop :=
 .
 
 Definition is_itree_retval {E A} tree a := @is_itree_retval' E A (observe tree) a.
-
-
-Infix ">>=" := ITree.bind (at level 58, left associativity).
-Notation "m1 >> m2" := (m1 >>= fun _ => m2) (at level 58, left associativity).
 
 Instance Proper_observing_is_itree_retval E A :
   Proper (observing eq ==> eq ==> iff) (@is_itree_retval E A).
@@ -536,6 +799,81 @@ Proof.
       rewrite <- (observing_intros _ _ _ e_obsm). assumption. }
 Qed.
 
+Notation " x : T <- m1 ;; m2" := (ITree.bind m1 (fun x : T=> m2) ) (at level 40).
+
+Section l_bind_satisfies_bind_counter.
+  Variant NonDet : Type -> Type := Choose : NonDet bool.
+
+  Definition m_counter : itree NonDet unit := 
+    x : bool <- ITree.trigger Choose ;; 
+    if x then Ret tt else y : bool <- ITree.trigger Choose;; Ret tt.
+
+  Definition P_counter : itree_spec NonDet unit :=
+    x : bool <- ITree.trigger (Spec_vis Choose);; Ret tt.
+
+  Definition Q_counter : unit -> itree_spec NonDet unit :=
+    fun _ => or_spec (Ret tt) ( x : bool <- ITree.trigger (Spec_vis Choose);; Ret tt  ).
+
+  Lemma m_counter_sats_P_bind_Q_counter : satisfies (P_counter >>= Q_counter) m_counter.
+  Proof.
+    pfold. red. cbn. constructor. left. destruct x.
+    - pfold. red. cbn.
+      assert (RetF (E:= NonDet) tt = observe (Ret tt)); auto.
+      rewrite H. constructor. exists true. left. pfold; constructor.
+    - pfold. red. cbn. assert (VisF Choose (fun x : bool => _ : bool <- Ret x;; Ret tt) = 
+                               observe (Vis Choose (fun x : bool => _ : bool <- Ret x;; Ret tt) ) ); auto.
+      rewrite H. constructor. exists false. left. pfold. red. cbn.
+      rewrite H. constructor. intros [ | ]; left; pfold; red; cbn; auto.
+   Qed.
+
+  Lemma satifies_P_counter : forall m, satisfies P_counter m -> 
+                                  m ≈ (x : bool <- ITree.trigger Choose;; Ret tt).
+  Proof.
+    intros. unfold P_counter in *. punfold H. red in H. pfold. red. cbn in *.
+    dependent induction H.
+    - rewrite <- x. constructor; auto.
+    - rewrite <- x. constructor. left. pclearbot. specialize (H v).
+      assert (satisfies (_ : bool <- Ret v;; Ret tt) (tree v) ); auto.
+      enough (tree v ≈ ( _ : bool <- Ret v;; Ret tt) ); auto. rewrite bind_ret_l.
+      rewrite bind_ret_l in H0. symmetry. clear x H m.
+      pfold. red. punfold H0. red in H0. cbn in *.
+      remember (observe (tree v) ) as ot. clear Heqot tree v. dependent induction H0; auto.
+  Qed.
+
+  Definition m0_counter : itree NonDet unit := x : bool <- ITree.trigger Choose;; Ret tt.
+
+  Lemma m0_counter_no_continuation : forall k,
+      ~ m0_counter >>= k ≈ m_counter .
+  Proof.
+    unfold m0_counter, m_counter.
+    intros k Hcontra. repeat rewrite bind_trigger in Hcontra.
+    rewrite bind_vis in Hcontra. apply eqit_inv_vis in Hcontra as [_ Hcontra] .
+    specialize (Hcontra true) as Hktrue. specialize (Hcontra false) as Hkfalse.
+    cbn in *. rewrite bind_ret_l in Hktrue. rewrite bind_ret_l in Hkfalse.
+    rewrite Hktrue in Hkfalse. pinversion Hkfalse.
+  Qed.
+
+  Lemma not_l_bind_satisfies_bind_aux : exists E R S 
+               (m : itree E R) (P : itree_spec E S) (Q : S -> itree_spec E R),
+      satisfies (P >>= Q) m /\ (forall m0 k, satisfies P m0 -> ~ (m0 >>= k ≈ m) ).
+    Proof.
+      exists NonDet, unit, unit, m_counter, P_counter, Q_counter. 
+      split; try apply m_counter_sats_P_bind_Q_counter.
+      intros. apply satifies_P_counter in H. rewrite H. fold m0_counter.
+      apply m0_counter_no_continuation.
+    Qed.
+
+
+End l_bind_satisfies_bind_counter.
+
+Lemma not_l_bind_satisfies_bind : ~ forall E R S 
+            (m : itree E R) (P : itree_spec E S) (Q : S -> itree_spec E R),
+       satisfies (P >>= Q) m -> exists m0 k, satisfies P m0 /\ (forall a, is_itree_retval m0 a -> satisfies (Q a) (k a) ) /\ (m0 >>= k ≈ m).
+Proof.
+  destruct not_l_bind_satisfies_bind_aux as [ E [R [S [m [P [Q  [H0 H1] ] ] ] ] ] ].
+  intros Hcontra. specialize (Hcontra E R S m P Q H0).
+  destruct Hcontra as [m0 [k [Hsat [ _ Heutt] ] ] ]. eapply H1; eauto. 
+Qed.
 
 (* Our event type = errors *)
 Inductive CompMEvent : Type -> Type :=
